SelfConnectEval.dfy
@@ -8,6 +8,7 @@ module SelfConnectEval {
   import opened Subcircuit
   import opened ConservedSubcircuit
   import opened SelfConnectEval2
+  import opened Path
 
   ghost predicate ConnectRequirements(c: Circuit, s: Scuf, conn: InternalConnection, fi: FI)
   {
@@ -32,6 +33,9 @@ module SelfConnectEval {
       && FIValid(fi, new_s.mp.inputs, new_s.mp.state)
       && s.SomewhatValidRelaxInputs(new_c)
       && new_s.SomewhatValidRelaxInputs(new_c)
+      && var conn_outputs := conn.GetConnectedOutputs(s.mp);
+      && var conn_inputs := conn.GetConnectedInputs(s.mp);
+      && !PathExistsBetweenNPSets(new_c, conn_outputs, conn_inputs)
     ensures
       var (new_c, new_s) := ConnectCircuitScufImpl(c, s, conn);
       && FICircuitValid(new_c, fi)
@@ -88,5 +92,84 @@ module SelfConnectEval {
     }
 
   }
+
+  function ConnectCircuitScuf(c: Circuit, s: Scuf, conn: InternalConnection): (r: (Circuit, Scuf))
+    requires c.Valid()
+    requires s.Valid(c)
+    requires conn.Valid()
+    requires ScufConnectionConsistent(c, s, conn)
+    ensures
+      var (new_c, new_s) := r;
+      && new_c.Valid()
+      && new_s.Valid(new_c)
+      && s.ValidRelaxInputs(new_c)
+  {
+    reveal ScufConnectionConsistent();
+    var (new_c, new_s) := ConnectCircuitScufImpl(c, s,conn);
+    assert new_s.Valid(new_c) by {
+      assert ScValid(new_c, s.sc) by {
+        assert ScValid(c, s.sc);
+        reveal ScValid();
+        assert new_c.NodeKind == c.NodeKind;
+      }
+      assert new_s.SomewhatValid(new_c) by {
+      }
+      assert new_s.SomewhatValidRelaxInputs(new_c) by {
+        new_s.SomewhatValidToRelaxInputs(new_c);
+      }
+      assert new_s.EvaluatesCorrectly(new_c) by {
+        reveal ScValid();
+        ScufFOutputsAreValid(new_c, new_s);
+        reveal Seq.ToSet();
+        forall fi: FI | FIValid(fi, new_s.mp.inputs, new_s.mp.state)
+          ensures forall np :: np in Seq.ToSet(new_s.mp.outputs) || np in StateINPs(new_s.mp.state) ==>
+            && FICircuitValid(new_c, fi)
+            && (Evaluate(new_c, np, fi) == EvalOk(MFLookup(new_s, fi, np)))
+        {
+          assert FICircuitValid(new_c, fi) by {ScufValidFiValidToFICircuitValid(new_c, new_s, fi);}
+          forall np | np in Seq.ToSet(new_s.mp.outputs) || np in StateINPs(new_s.mp.state)
+            ensures Evaluate(new_c, np, fi) == EvalOk(MFLookup(new_s, fi, np))
+          {
+            reveal ScufConnectionConsistent();
+            var conn_outputs := conn.GetConnectedOutputs(s.mp);
+            var conn_inputs := conn.GetConnectedInputs(s.mp);
+            ScufFInputsAreValid(c, s);
+            ScufFOutputsAreValid(c, s);
+            reveal ONPsValid();
+            StillNoPathExistsBetweenNPSets(c, new_c, conn_outputs, conn_inputs);
+            EvaluateSelfConnect(c, s, conn, np, fi);
+          }
+        }
+        reveal Scuf.EvaluatesCorrectly();
+      }
+      assert new_s.MapValid() by {
+      }
+    }
+    assert s.ValidRelaxInputs(new_c) by {
+      assert s.MapValid();
+      assert ScValid(new_c, s.sc);
+      assert s.SomewhatValidRelaxInputs(new_c);
+      reveal Scuf.EvaluatesCorrectly();
+      assert s.EvaluatesCorrectly(new_c) by {
+        reveal ScValid();
+        ScufFOutputsAreValid(new_c, s);
+        reveal Seq.ToSet();
+        forall fi: FI | FIValid(fi, s.mp.inputs, s.mp.state)
+          ensures forall np :: np in Seq.ToSet(s.mp.outputs) || np in StateINPs(s.mp.state) ==>
+            && FICircuitValid(new_c, fi)
+            && (Evaluate(new_c, np, fi) == EvalOk(MFLookup(s, fi, np)))
+        {
+          assert FICircuitValid(new_c, fi) by {ScufValidFiValidToFICircuitValid(new_c, s, fi);}
+          forall np | np in Seq.ToSet(s.mp.outputs) || np in StateINPs(s.mp.state)
+            ensures Evaluate(new_c, np, fi) == EvalOk(MFLookup(s, fi, np))
+          {
+            EvaluateSelfConnectOldONP(c, s, conn, np, fi);
+          }
+        }
+      }
+    }
+    (new_c, new_s)
+  }
+
 
 }
